bring everything up to date with the latest changes in semantics

AbstractAnalysis.v
@@ -1,46 +1,76 @@
-Require Import Machine.
-Require Import BoundedLattice.
-Require Import Coq.Lists.List. 
+Require Import VerifiedVerifier.Machine.
+Require Import VerifiedVerifier.BoundedLattice.
+Require Import VerifiedVerifier.BinaryLattice.
+Require Import VerifiedVerifier.Maps.
+Require Import Coq.Lists.List.
 
+Record info := {
+  abs_heap_base : BinarySet;
+  abs_heap_bound : BinarySet;
+  abs_cf_bound : BinarySet;
+}.
+
+Definition empty_info :=
+  {| abs_heap_base := top;
+     abs_heap_bound := top;
+     abs_cf_bound := top; |}.
+
+Definition abs_heap_base_info :=
+  {| abs_heap_base := bottom;
+     abs_heap_bound := top;
+     abs_cf_bound := top; |}.
+
+Definition abs_heap_bounded_info :=
+  {| abs_heap_base := top;
+     abs_heap_bound := bottom;
+     abs_cf_bound := top; |}.
+
+Definition abs_cf_bounded_info :=
+  {| abs_heap_base := top;
+     abs_heap_bound := top;
+     abs_cf_bound := bottom; |}.
+
+(*
 Record absStateLattice := {
-  heap_base         : BoundedSet;
+  abs_heap_base         : BoundedSet;
   heap              : BoundedSet;
   fn_table          : BoundedSet;
 }.
 
 Definition unbounded_lattice :=
-  {| heap_base := top;
+  {| abs_heap_base := top;
      heap := top;
      fn_table := top; |}.
 
-Definition heap_base_bounded_lattice :=
-  {| heap_base := bounded;
+Definition abs_heap_base_bounded_lattice :=
+  {| abs_heap_base := bounded;
      heap := top;
      fn_table := top; |}.
 
-Definition heap_bounded_lattice :=
-  {| heap_base := top;
+Definition abs_heap_bounded_lattice :=
+  {| abs_heap_base := top;
      heap := bounded;
      fn_table := top; |}.
 
 Definition fn_table_bounded_lattice :=
-  {| heap_base := top;
+  {| abs_heap_base := top;
      heap := top;
      fn_table := bounded; |}.
 
 Definition absStateLattice_join (a : absStateLattice) (b : absStateLattice) : absStateLattice :=
-  {| heap_base := join_BoundedSet a.(heap_base) b.(heap_base);
+  {| abs_heap_base := join_BoundedSet a.(abs_heap_base) b.(abs_heap_base);
      heap := join_BoundedSet a.(heap) b.(heap);
      fn_table := join_BoundedSet a.(fn_table) b.(fn_table) |}.
 
 Definition absStateLattice_meet (a : absStateLattice) (b : absStateLattice) : absStateLattice :=
-  {| heap_base := meet_BoundedSet a.(heap_base) b.(heap_base);
+  {| abs_heap_base := meet_BoundedSet a.(abs_heap_base) b.(abs_heap_base);
      heap := meet_BoundedSet a.(heap) b.(heap);
      fn_table := meet_BoundedSet a.(fn_table) b.(fn_table) |}.
+*)
 
-Definition abs_registers_ty := fmap register absStateLattice.
+Definition abs_registers_ty := total_map register info.
 
-Definition abs_stack_ty := list absStateLattice.
+Definition abs_stack_ty := list info.
 
 (* Definition heap_ty := list lattice.*)
 
@@ -55,8 +85,8 @@ Record abs_state := {
 
 Definition abs_empty_state :=
 {| abs_regs := fun r => if register_eq_dec r rdi
-                          then heap_base_bounded_lattice
-                          else unbounded_lattice;
+                          then abs_heap_base_info
+                          else empty_info;
    abs_stack := nil;
 (*   heap := nil *)|}.
 
@@ -100,7 +130,7 @@ Definition set_flags (s : machine) (f : flags_ty) : machine :=
 Definition expand_abs_stack (s : abs_state) (i : nat) : abs_state :=
 {| abs_regs := s.(abs_regs);
 (*   flags := s.(flags); *)
-   abs_stack := s.(abs_stack) ++ (repeat unbounded_lattice i);
+   abs_stack := s.(abs_stack) ++ (repeat empty_info i);
 (*   heap := s.(heap) *)|}.
 
 Fixpoint contract_abs_stack (s : abs_state) (i : nat) : abs_state :=
@@ -146,21 +176,21 @@ Next Obligation. rewrite <- plus_n_O. repeat (rewrite <- plus_n_Sm). reflexivity
 Qed.
 *)
 
-Definition get_register_lattice (s : abs_state) (r : register) : absStateLattice :=
-  map_get s.(abs_regs) r.
+Definition get_register_info (s : abs_state) (r : register) : info :=
+  s.(abs_regs) r.
 
-Definition set_register_lattice (s : abs_state) (r : register) (l : absStateLattice) : abs_state :=
-{| abs_regs := map_set register_eq_dec s.(abs_regs) r l;
+Definition set_register_info (s : abs_state) (r : register) (i : info) : abs_state :=
+{| abs_regs := t_update register_eq_dec s.(abs_regs) r i;
    abs_stack := s.(abs_stack);
 (*   heap := s.(heap) *) |}.
 
-Definition get_stack_lattice (s : abs_state) (index : nat) : absStateLattice :=
-nth index s.(abs_stack) unbounded_lattice.
+Definition get_stack_info (s : abs_state) (index : nat) : info :=
+nth index s.(abs_stack) empty_info.
 
 (* this needs to be updated *)
-Definition set_stack_lattice (s : abs_state) (index : nat) (l : absStateLattice) : abs_state :=
+Definition set_stack_info (s : abs_state) (index : nat) (i : info) : abs_state :=
 {| abs_regs := s.(abs_regs);
-   abs_stack := update s.(abs_stack) index l;
+   abs_stack := Machine.update s.(abs_stack) index i;
  (*  heap := s.(heap) *) |}.
 
 Definition empty {A} (l : list A) :=
@@ -173,22 +203,22 @@ Reserved Notation " i '/' st 'v-->' st' "
 Inductive instr_class_vstep : instr_class -> abs_state -> abs_state -> Prop := 
 | V_Heap_Read: forall st r_base r_src r_dst,
     (* r_base <> r_src -> *) (* not sure if we need this to make the proofs easier *)
-    (get_register_lattice st r_base).(heap_base) = bounded ->
-    (get_register_lattice st r_src).(heap) = bounded ->
-    Heap_Read r_dst r_src r_base / st v--> (set_register_lattice st r_dst unbounded_lattice) 
+    (get_register_info st r_base).(abs_heap_base) = bottom ->
+    (get_register_info st r_src).(abs_heap_bound) = bottom ->
+    Heap_Read r_dst r_src r_base / st v--> (set_register_info st r_dst empty_info) 
 | V_Heap_Write: forall st r_base r_src r_dst,
     (* r_base <> r_src -> *) (* not sure if we need this to make the proofs easier *)
-    (get_register_lattice st r_base).(heap_base) = bounded ->
-    (get_register_lattice st r_dst).(heap) = bounded -> 
+    (get_register_info st r_base).(abs_heap_base) = bottom ->
+    (get_register_info st r_dst).(abs_heap_bound) = bottom -> 
     Heap_Write r_dst r_src r_base / st v--> st
 | V_Heap_Check: forall st r_src,
-    Heap_Check r_src / st v--> (set_register_lattice st r_src heap_bounded_lattice)
+    Heap_Check r_src / st v--> (set_register_info st r_src abs_heap_bounded_info)
 | V_Call_Check: forall st r_src,
-    Call_Check r_src / st v--> (set_register_lattice st r_src fn_table_bounded_lattice)
+    Call_Check r_src / st v--> (set_register_info st r_src abs_cf_bounded_info)
 | V_Reg_Move: forall st r_src r_dst,
-    Reg_Move r_dst r_src / st v--> (set_register_lattice st r_dst (get_register_lattice st r_src))
+    Reg_Move r_dst r_src / st v--> (set_register_info st r_dst (get_register_info st r_src))
 | V_Reg_Write: forall st r_dst val,
-    Reg_Write r_dst val / st v--> (set_register_lattice st r_dst unbounded_lattice)
+    Reg_Write r_dst val / st v--> (set_register_info st r_dst empty_info)
 | V_Stack_Expand: forall st i,
     Stack_Expand i / st v--> (expand_abs_stack st i)
 | V_Stack_Contract: forall st i,
@@ -196,17 +226,25 @@ Inductive instr_class_vstep : instr_class -> abs_state -> abs_state -> Prop :=
     Stack_Contract i / st v--> (contract_abs_stack st i)
 | V_Stack_Read: forall st i r_dst,
     i < (length st.(abs_stack)) ->
-    Stack_Read r_dst i / st v--> (set_register_lattice st r_dst (get_stack_lattice st i))
+    Stack_Read r_dst i / st v--> (set_register_info st r_dst (get_stack_info st i))
 | V_Stack_Write: forall st i r_src,
     i < (length st.(abs_stack)) ->
-    Stack_Write i r_src / st v--> (set_stack_lattice st i (get_register_lattice st r_src))
+    Stack_Write i r_src / st v--> (set_stack_info st i (get_register_info st r_src))
 | V_Indirect_Call: forall st reg,
-    (get_register_lattice st reg).(fn_table) = bounded ->
-    (get_register_lattice st rdi).(heap_base) = bounded ->
+    (get_register_info st reg).(abs_cf_bound) = bottom ->
+    (get_register_info st rdi).(abs_heap_base) = bottom ->
     Indirect_Call reg / st v-->  st
 | V_Direct_Call: forall st str,
-    (get_register_lattice st rdi).(heap_base) = bounded ->
+    (get_register_info st rdi).(abs_heap_base) = bottom ->
     Direct_Call str / st v-->  st
+| V_Branch: forall st cond, 
+    Branch cond / st v--> st
+| V_UniOp: forall st op r_dst,
+    UniOp op r_dst / st v--> (set_register_info st r_dst empty_info)
+| V_BinOp: forall st op r_dst r_src,
+    BinOp op r_dst r_src / st v--> (set_register_info st r_dst empty_info)
+| V_DivOp: forall st r_dst,
+    DivOp r_dst / st v--> (set_register_info (set_register_info st rax empty_info) r_dst empty_info)
 | V_Ret: forall st,
     empty st.(abs_stack) ->
     Ret / st v-->  st
@@ -250,36 +288,34 @@ Proof.
   eexists. eapply multi_step.
   - apply I_Basic_Block. apply V_Heap_Check.
   - eapply multi_step.
-    + apply I_Basic_Block. apply V_Heap_Read.
-      * unfold map_set. auto.
-      * unfold map_set. auto.
+    + apply I_Basic_Block. apply V_Heap_Read; auto.
     + apply multi_refl.
 Qed.
 
 Lemma register_get_after_set_eq : forall (abs_regs : abs_registers_ty) reg v,
-    map_get (map_set register_eq_dec abs_regs reg v) reg = v.
+  (t_update register_eq_dec abs_regs reg v) reg = v.
 Proof.
-  intros abs_regs reg v. unfold map_get. unfold map_set. destruct (register_eq_dec reg reg).
+  intros abs_regs reg v. unfold t_update. destruct (register_eq_dec reg reg).
   - reflexivity.
   - exfalso. apply n. reflexivity.
 Qed.
 
 Lemma register_get_after_set_neq : forall (abs_regs : abs_registers_ty) reg1 reg2 v,
     reg1 <> reg2 ->
-    map_get (map_set register_eq_dec abs_regs reg2 v) reg1 = map_get abs_regs reg1.
+    (t_update register_eq_dec abs_regs reg2 v) reg1 = abs_regs reg1.
 Proof.
-  intros abs_regs reg1 reg2 v Heq. unfold map_get. unfold map_set. destruct (register_eq_dec reg2 reg1).
+  intros abs_regs reg1 reg2 v Heq. unfold t_update. destruct (register_eq_dec reg2 reg1).
   - exfalso. apply Heq. auto.
   - reflexivity.
 Qed.
 
 Definition safe_stack_read (st : abs_state) (r_base : register) (r_src : register) (r_dst : register) : Prop :=
-  r_base <> r_src /\ (get_register_lattice st r_base).(heap_base) = bounded
-                  /\ (get_register_lattice st r_src).(heap) = bounded.
+  r_base <> r_src /\ (get_register_info st r_base).(abs_heap_base) = bottom
+                  /\ (get_register_info st r_src).(abs_heap_bound) = bottom.
 
 Lemma read_after_check_is_safe: forall r_base r_src r_dst st, exists st' st'',
   r_base <> r_src ->
-  (get_register_lattice st r_base).(heap_base) = bounded ->
+  (get_register_info st r_base).(abs_heap_base) = bottom ->
   Heap_Check r_src / st v--> st' /\ Heap_Read r_dst r_src r_base / st' v--> st''.
 Proof.
   intros r_base r_src r_dst st. 
@@ -287,8 +323,10 @@ Proof.
   split.
   - apply V_Heap_Check.
   - apply V_Heap_Read.
-    + unfold get_register_lattice in *. unfold set_register_lattice. simpl.
+    + unfold get_register_info in *. unfold set_register_info. simpl.
       rewrite register_get_after_set_neq; auto.
-    + unfold get_register_lattice in *. unfold set_register_lattice. simpl.
+    + unfold get_register_info in *. unfold set_register_info. simpl.
       rewrite register_get_after_set_eq; auto.
 Qed.
+
+
