BinaryLattice.v
@@ -1,0 +1,89 @@
+Require Import VerifiedVerifier.Lattice.
+
+Inductive BinarySet : Set :=
+| top 
+| bottom.
+
+Inductive BinaryRel : BinarySet -> BinarySet -> Prop :=
+| bot_rel x : BinaryRel bottom x
+| top_rel x : BinaryRel x top.
+
+Program Instance BinaryOrder : Order BinarySet := { ord := BinaryRel }.
+Next Obligation.
+  unfold RelationClasses.Reflexive.
+  intros x. destruct x. apply top_rel. apply bot_rel. 
+Defined.
+Next Obligation. Proof.
+  induction x; induction y; auto; inversion H; inversion H0.
+Defined.
+Next Obligation. Proof.
+  unfold RelationClasses.Transitive.
+  induction x; induction y; induction z; auto; intros; try apply self_rel;
+    try inversion H; try inversion H0.
+Defined.
+
+Definition meet_BinarySet (a : BinarySet) (b : BinarySet) : BinarySet :=
+  match a with
+  | top => b
+  | bottom => bottom
+  end.
+
+Definition join_BinarySet (a : BinarySet) (b : BinarySet) : BinarySet :=
+  match a with
+  | bottom => b
+  | top => top
+  end.
+
+Program Instance BinaryLattice : Lattice BinarySet :=
+  {
+    meet := meet_BinarySet;
+    join := join_BinarySet;
+
+    (*meet_commutative : forall a b, a ⊓ b = b ⊓ a;
+    meet_associative : forall a b c, (a ⊓ b) ⊓ c = a ⊓ (b ⊓ c);
+    meet_absorptive  : forall a b, a ⊓ (a ⊔ b) = a;
+    meet_idempotent  : forall a, a ⊓ a = a;
+
+    join_commutative : forall a b, a ⊔ b = b ⊔ a;
+    join_associative : forall a b c, (a ⊔ b) ⊔ c = a ⊔ (b ⊔ c);
+    join_absorptive  : forall a b, a ⊔ (a ⊓ b) = a;
+    join_idempotent  : forall a, a ⊔ a = a*)
+  }.
+Next Obligation.
+  unfold meet_BinarySet; induction a; induction b; auto.
+Defined.
+Next Obligation. Proof.
+  unfold meet_BinarySet; induction a; induction b; induction c; auto.
+Defined.
+Next Obligation. Proof.
+  unfold meet_BinarySet; unfold join_BinarySet; induction a; induction b; auto.
+Defined.
+Next Obligation. Proof.
+  unfold meet_BinarySet; induction a; auto.
+Defined.
+Next Obligation. Proof.
+  unfold join_BinarySet; induction a; induction b; auto.
+Defined.
+Next Obligation. Proof.
+  unfold join_BinarySet; induction a; induction b; induction c; auto.
+Defined.
+Next Obligation. Proof.
+  unfold join_BinarySet; unfold meet_BinarySet; induction a; induction b; auto.
+Defined.
+Next Obligation. Proof.
+  unfold join_BinarySet; induction a; auto.
+Defined.
+
+Program Instance BinaryLOSet : LOSet BinaryOrder BinaryLattice.
+Next Obligation.
+  split.
+  - intros. induction a; induction b; auto; unfold meet_BinarySet; inversion H.
+  - intros. induction a; induction b; auto; unfold meet_BinarySet in H; inversion H;
+    try apply bot_rel; try apply top_rel.
+Defined.
+Next Obligation. Proof.
+  split.
+  - intros. induction a; induction b; auto; unfold join_BinarySet; inversion H.
+  - intros. induction a; induction b; auto; unfold join_BinarySet in H; inversion H;
+    try apply bot_rel; try apply top_rel.
+Defined.
