Maps.v
@@ -1,0 +1,144 @@
+Definition total_map (A B:Type) := 
+  A -> B.
+
+Definition t_update {A B : Type} (eq_dec:forall (x y:A),{x=y}+{x<>y}) (f:total_map A B) (x:A) (v:B) : total_map A B :=
+  fun y => if eq_dec x y then v else f y.
+
+Definition t_get {A} {B} (f:total_map A B) (x:A) : B := 
+  f x.
+
+Definition t_empty {A} {B} (v:B) : total_map A B :=
+  fun (_ : A) => v.
+
+
+Lemma t_apply_empty: forall A B x v, @t_empty A B v x = v.
+Proof.
+  intros.
+  unfold t_empty. reflexivity.
+Qed.
+
+(*
+Lemma t_update_eq : forall A B eq_dec (m: total_map A B) x v,
+  (t_update eq_dec m x v) x = v.
+Proof.
+  intros.
+  unfold t_update.
+  rewrite <- beq_id_refl.
+  reflexivity.
+Qed.
+
+Theorem t_update_neq : forall (X:Type) v x1 x2
+                         (m : total_map X),
+  x1 <> x2 ->
+  (t_update m x1 v) x2 = m x2.
+Proof.
+  intros.
+  apply false_beq_id in H.
+  unfold t_update.
+  rewrite -> H.
+  reflexivity.
+Qed.
+
+Lemma t_update_shadow : forall A (m: total_map A) v1 v2 x,
+    t_update (t_update m x v1) x v2
+  = t_update m x v2.
+Proof.
+  intros.
+  unfold t_update.
+  apply functional_extensionality_dep.
+  intros.
+  destruct (beq_id x x0).
+  + reflexivity.
+  + reflexivity.
+Qed.
+
+Theorem t_update_same : forall X x (m : total_map X),
+  t_update m x (m x) = m.
+Proof.
+  intros.
+  unfold t_update.
+  apply functional_extensionality_dep.
+  intros.
+  destruct (beq_idP x x0).
+  + rewrite -> e. reflexivity.
+  + reflexivity.
+Qed.
+
+Theorem t_update_permute : forall (X:Type) v1 v2 x1 x2
+                             (m : total_map X),
+  x2 <> x1 ->
+    (t_update (t_update m x2 v2) x1 v1)
+  = (t_update (t_update m x1 v1) x2 v2).
+Proof.
+  intros.
+  unfold t_update.
+  apply functional_extensionality_dep.
+  intros.
+  destruct (beq_idP x1 x).
+  - destruct (beq_idP x2 x).
+    + exfalso. apply H. rewrite e, e0. reflexivity.
+    + reflexivity.
+  - destruct (beq_idP x2 x).
+    + reflexivity.
+    + reflexivity.
+Qed.
+*)
+
+Definition partial_map (A B:Type) := total_map A (option B).
+
+Definition empty {A B: Type} : partial_map A B :=
+  t_empty None.
+
+Definition update {A B: Type} (eq_dec:forall (x y:A),{x=y}+{x<>y}) (m: partial_map A B) (k: A) (v: B) :=
+  t_update eq_dec m k (Some v).
+
+Definition member {A B: Type} (m : partial_map A B) (k: A) :=
+match (m k) with
+| Some _ => true
+| None => false
+end.
+
+Lemma apply_empty : forall A B x, @empty A B x = None.
+Proof.
+  intros. unfold empty. rewrite t_apply_empty. reflexivity.
+Qed.
+
+(*
+Lemma update_eq : forall A B eq_dec (m: partial_map A B) x v,
+  (update eq_dec m x v) x = Some v.
+Proof.
+  intros. unfold update. rewrite t_update_eq. reflexivity.
+Qed.
+
+Lemma update_neq : forall A (m: partial_map A) x1 x2 v,
+  x2 <> x1 ->
+  (update m x2 v) x1 = m x1.
+Proof.
+  intros. unfold update. rewrite t_update_neq.
+  - reflexivity.
+  - apply H.
+Qed.
+
+Lemma update_shadow : forall A (m: partial_map A) x v1 v2,
+  update (update m x v1) x v2 = update m x v2.
+Proof.
+  intros. unfold update. rewrite t_update_shadow. reflexivity.
+Qed.
+
+Lemma update_same : forall A (m: partial_map A) x v,
+  m x = Some v ->
+  update m x v = m.
+Proof.
+  intros. unfold update. rewrite <- H. rewrite t_update_same. reflexivity.
+Qed.
+
+Lemma update_permute : forall A (m: partial_map A) x1 x2 v1 v2,
+  x2 <> x1 ->
+  (update (update m x2 v2) x1 v1) =
+  (update (update m x1 v1) x2 v2).
+Proof.
+  intros. unfold update. rewrite t_update_permute.
+  - reflexivity.
+  - apply H.
+Qed.
+*)
